q

qr.ec
@@ -1,5 +1,5 @@
 pragma Goals:printall.
-require import AllCore DBool Bool List Distr.
+require import AllCore DBool Bool List Distr Int IntDiv.
 
 
 (* https://crypto.stanford.edu/pbc/notes/numbertheory/qr.html *)
@@ -9,23 +9,36 @@ replace IsQR with IsSqRoot ((N, y), w)
 add invertability assumption into qr_prop7
 *)
 
-op sqDist :  int -> int distr. 
-op sqRoot :  int -> int -> int.
+op ZNS_dist :  int -> (int * int) distr.     (* ZN* *)
 op inv : int -> int -> int.
-op IsQR : int -> int -> bool.
+op invertible : int -> int -> bool.
 
-axiom sqDistr_uni N :  is_uniform (sqDist N).
-axiom sqDist_prop0 N x : IsQR N x => x \in sqDist N.
-axiom sqDist_prop N x : x \in sqDist N => IsQR N x.
-axiom qr_prop (N x : int) : IsQR N x => (sqRoot N x) * (sqRoot N x) = x.
-axiom qr_prop1 (N x : int) : IsQR N x => x * (inv N x) = 1.
-axiom qr_prop2 (N x : int) : IsQR N x => IsQR N (inv N x).
-axiom qr_prop3 (N x y : int) : IsQR N x => IsQR N y => IsQR N (x * y).
-axiom qr_prop4 (N : int) : sqRoot N 1 = 1.
-axiom qr_prop5 (N x y : int) : IsQR N x => IsQR N y => 
-   sqRoot N (x * y) = sqRoot N x * sqRoot N y. 
-axiom qr_prop6 (N x y r : int) : IsQR N x => !IsQR N y => (x * y) <> r * r.
-axiom qr_prop7 (N y r : int) : !IsQR N y => y <> r * r.
+op IsSqRoot (N y w : int) = y %% N  = (w * w) %% N. 
+op IsQR (N y : int) = exists w, IsSqRoot N y w.
+
+
+axiom d_prop1 N r rr :  (r, rr) \in ZNS_dist N => r * r %% N = rr %% N.
+axiom d_prop2 N r rr :  (r, rr) \in ZNS_dist N => (r, rr) = (r %% N, rr %% N).
+
+
+
+
+(* axiom sqDistr_uni N :  is_uniform (sqDist N). *)
+(* axiom sqDist_prop0 N x : IsQR N x => x \in sqDist N. *)
+(* axiom sqDist_prop N x : x \in sqDist N => IsQR N x. *)
+(* axiom qr_prop (N x : int) : IsQR N x => (sqRoot N x) * (sqRoot N x) = x. *)
+(* axiom qr_prop1 (N x : int) : IsQR N x => x * (inv N x) = 1. *)
+(* axiom qr_prop2 (N x : int) : IsQR N x => IsQR N (inv N x). *)
+(* axiom qr_prop3 (N x y : int) : IsQR N x => IsQR N y => IsQR N (x * y). *)
+(* axiom qr_prop4 (N : int) : sqRoot N 1 = 1. *)
+(* axiom qr_prop5 (N x y : int) : IsQR N x => IsQR N y =>  *)
+(*    sqRoot N (x * y) = sqRoot N x * sqRoot N y.  *)
+axiom qr_prop6 (N x y r : int) : IsQR N x => !IsQR N y => x * y %% N <> r * r %% N.
+axiom qr_prop1 (N x : int) : invertible N x => x * (inv N x) %% N = 1.
+axiom qr_prop11 (N x : int) : invertible N x => (inv N x) * x  %% N = 1.
+axiom qr_prop2 (N x y w : int) : invertible N y => IsSqRoot N y w => invertible N w.
+axiom qr_prop3 (N x y w : int) : invertible N y => IsSqRoot N y w => IsQR N w.
+(* axiom qr_prop7 (N y r : int) : !IsQR N y => y <> r * r. *)
 
 
 
@@ -35,10 +48,9 @@ axiom qr_prop7 (N y r : int) : !IsQR N y => y <> r * r.
 - wants to convinvce the verifier that he knows the proof
 *)
 module type Prover = {
-  proc commit(N : int, y : int) : int
+  proc commit(N : int, y : int, w : int) : int
   proc response(b : bool) : int
 }.
-
 
 module type Verifier = {
   proc challenge(N : int, y : int, c : int) : bool  
@@ -62,8 +74,8 @@ module type Simulator = {
 module Correct(P : Prover, V : Verifier) = {
   var c, r : int
   var b, result : bool
-  proc main(N : int, y : int) = {
-    c <- P.commit(N, y);  
+  proc main(N : int, y : int, w : int) = {
+    c <- P.commit(N, y,w);  
     b <- V.challenge(N,y,c);
     r <- P.response(b);
     result <- V.verify(c,b,r);  
@@ -73,16 +85,16 @@ module Correct(P : Prover, V : Verifier) = {
 
 (* honest prover  *)
 module HP : Prover = {
-  var rr, n, y : int
+  var r,rr, n, y, w : int
 
-  proc commit(n1 : int, y1 : int) : int = {  
-    (n,y) <- (n1, y1);
-    rr <$ sqDist n;
+  proc commit(n1 : int, y1 : int, w1 : int) : int = {  
+    (n,y,w) <- (n1, y1, w1);
+    (r,rr) <$ ZNS_dist n;
     return rr;
   }
 
   proc response(b : bool) : int = {
-    return (sqRoot n rr) * (if b then (sqRoot n y) else 1);
+    return (r * (if b then w else 1)) %% n;
  } 
 }.
 
@@ -98,18 +110,25 @@ module HV : Verifier = {
   }
 
   proc verify(c : int,b : bool, r : int) : bool = {
-    return (if b then c * y = r * r else c = r * r);
+    return (if b then (c * y)  %% n = (r * r) %% n else (c %% n) = (r * r)%%n);
  } 
 }.
 
-
-lemma qrp_complete_ph Na ya : IsQR Na ya
-   => hoare [ Correct(HP,HV).main : arg = (Na,ya) ==> res ].
+lemma qrp_complete_ph Na ya wa : IsSqRoot Na ya wa
+   => hoare [ Correct(HP,HV).main : arg = (Na,ya,wa) ==> res ].
 move => qra.
 proc. inline*.  wp. 
 rnd. wp.  rnd.  wp. 
-skip. progress;smt.
+skip. progress.   
+ have f : y{hr} %% N{hr} = (w{hr} * w{hr}) %% N{hr}.
+apply qra. 
+clear qra.
+rewrite - (modzMml rrr.`2 y{hr} N{hr}).   
+rewrite -  (d_prop1 N{hr} rrr.`1 rrr.`2). smt.
+rewrite (modzMml (rrr.`1 * rrr.`1) y{hr} N{hr} ).
+smt (modzMml modzMmr modzMm). smt (d_prop1 modzMml modzMmr modzMm).
 qed.
+
 
 
 section.
@@ -119,24 +138,31 @@ axiom P_ax1 : islossless P.commit.
 axiom P_ax2 : islossless P.response.
 
 lemma qrp_sound Na ya :
- !IsQR Na ya => phoare [ Correct(P,HV).main : arg = (Na,ya) ==> res ] <= (1%r/2%r).
+ !IsQR Na ya => phoare [ Correct(P,HV).main : arg = (Na,ya,witness) ==> res ] <= (1%r/2%r).
 proof. move => qra.
 proc. inline*. 
 wp.
-seq 5 : ((N,y) = (Na,ya) /\ HV.y = y) (1%r) (1%r/2%r) (0%r) (1%r). auto.
+seq 5 : ((N,y) = (Na,ya) /\ HV.y = y /\ HV.n = N) (1%r) (1%r/2%r) (0%r) (1%r). auto.
 auto.
 exists* Correct.c. elim*. move => cv.
 case (!IsQR Na cv).
-seq 1 : (!b) (1%r/2%r) (0%r) (1%r/2%r) (1%r) (cv = Correct.c /\ (N,y) = (Na,ya) /\ HV.y = y /\ !IsQR Na cv).
+seq 1 : (!b) (1%r/2%r) (0%r) (1%r/2%r) (1%r) (cv = Correct.c /\ (N,y) = (Na,ya) /\ HV.y = y /\ HV.n = N /\ !IsQR Na cv).
 rnd.  skip. auto.
 hoare. call (_:true ==> true). auto.
-wp. auto. progress. rewrite H0. simplify.  smt (qr_prop7 ). 
+wp. auto. progress. rewrite H0. simplify.   
+have : forall (w : int), Correct.c{hr} %% N{hr} <> w * w %% N{hr}. clear qra H0. 
+   move => w.  
+
+  case (Correct.c{hr} %% N{hr} = w * w %% N{hr}). move => ass.
+  simplify. apply H. rewrite /IsQR. exists w. rewrite /IsSqRoot. apply ass. auto.
+progress. apply H1.
+
 simplify.
 rnd. skip. smt.
 conseq (_: _ ==> true). call (_: true ==> true). auto. 
 wp. skip. auto. auto.
   simplify.
-seq 1 : (b) (1%r/2%r) (0%r) (1%r/2%r) (1%r) (cv = Correct.c /\ (N,y) = (Na,ya) /\ IsQR Na cv /\ HV.y = y). 
+seq 1 : (b) (1%r/2%r) (0%r) (1%r/2%r) (1%r) (cv = Correct.c /\ (N,y) = (Na,ya) /\ IsQR Na cv /\ HV.y = y /\ HV.n = N). 
 rnd. skip. auto.
 hoare. 
 call (_:true ==> true). auto.  
@@ -146,10 +172,25 @@ rnd. skip. progress. smt.
 conseq (_: _ ==> true). call (_:true ==> true). auto.
 wp. skip. auto. auto.
 hoare.
-simplify. auto. call (_ : true ==> true).  auto.    skip. auto. auto.
+simplify. auto. call (_ : true ==> true).  auto. skip. auto. auto.
 qed.
 
 end section.
+
+
+
+  (* 
+  lemma nosmt modzMml: forall (m n d : int), m %% d * n %% d = m * n %% d.
+  lemma nosmt modzMmr: forall (m n d : int), m * (n %% d) %% d = m * n %% d.
+  lemma nosmt modzMm:
+    forall (m n d : int), m %% d * (n %% d) %% d = m * n %% d.
+  lemma nosmt modzNm: forall (m d : int), (- m %% d) %% d = (-m) %% d.
+  lemma nosmt mulz_modr:
+    forall (p m d : int), 0 < p => p * (m %% d) = p * m %% (p * d).
+  lemma nosmt mulz_modl:
+    forall (p m d : int), 0 < p => m %% d * p = m * p %% (d * p).
+
+ *)
 
 
 section.
@@ -161,18 +202,17 @@ local module Sim1  = {
   var result : bool list
 
   proc sinit(N : int, y : int) : bool * int * int = {
-    var rr,bb,zz;
+    var r,rr,bb;
+    (r,rr)  <$ ZNS_dist N;    
     bb <$ {0,1};
-    rr  <$ sqDist N;    
-    zz  <- rr * if bb then (inv N y) else 1;
-    return (bb,zz,rr);
+    return (bb,(rr * if bb then (inv N y) else 1) %% N,r);
   }
 
   proc simulate(N : int, y : int) : bool * bool list  = {
-    var rr,z,b',b,ryb;
-    (b',z,rr) <- sinit(N,y);
+    var r,z,b',b,ryb;
+    (b',z,r) <- sinit(N,y);
     b  <- V.challenge(N,y,z);   
-    ryb  <- (sqRoot N rr);
+    ryb  <- r %% N;
     result <- V.summitup(z,b,ryb); 
     return (b = b', result);    
   }
@@ -182,57 +222,174 @@ local module Sim1  = {
 local module Sim1'  = {
   var result : bool list
 
-  proc sinit(N : int, y : int) : bool * int = {
-    var rr,bb;
-    rr  <$ sqDist N;    
+  proc sinit(N : int, y : int) : bool * int * int  = {
+    var r,rr,bb;
+    (r,rr)  <$ ZNS_dist N;    
     bb <$ {0,1};
-    return (bb,rr);
+    return (bb,rr %% N,r);
   }
     
-  proc simulate(N : int, y : int) : bool * bool list  = {
-    var z,b',b,ryb,result;  
-    (b',z) <- sinit(N,y);    
+  proc simulate(N : int, y : int, w : int) : bool * bool list  = {
+    var z,r,b',b,ryb,result;
+    (b',z,r) <- sinit(N,y);
     b  <- V.challenge(N,y,z);
-    ryb  <- (sqRoot N (z * (if b then y else 1)));
-    result <- V.summitup(z,b,ryb); 
+    ryb  <- (r * if b then w else 1) %% N  ;
+    result <- V.summitup(z,b,ryb);
     return (b = b', result);
   }
 }.
 
 
-local lemma exss Na ya : IsQR Na ya =>
- equiv[ Sim1.sinit ~ Sim1'.sinit
-   : ={arg} /\ arg{1} = (Na,ya) ==>
-       (res{1}.`1, res{1}.`2) = res{2}
-        /\ (res{1}.`1 = true  => res{1}.`2 = res{1}.`3 * (inv Na ya))
-        /\ (res{1}.`1 = false => res{1}.`2 = res{1}.`3 /\ res{1}.`2 = res{2}.`2) ].
-move => isqr. proc. swap {2} 1 1.
-seq 1 1 : (={N,y,bb} /\ (N{1},y{1}) = (Na,ya)). rnd. skip. auto.
-exists* bb{1}. elim*. progress.
-wp. case (bb_L = true).
-rnd (fun x => x * (inv N{1} y{1})) (fun x => x * y{1}). skip. progress;smt.
-progress. rnd. skip. progress. smt.
+module ZK(P : Prover, V : VerifierA) = {
+  proc main(N : int, y : int, w : int) = {
+    var c,b,r,result;
+    c <- P.commit(N, y,w);
+    b <- V.challenge(N,y,c);
+    r <- P.response(b);
+    result <- V.summitup(c,b,r);
+    return result;
+  }
+}.
+
+
+local lemma qrp_zk2_eq Na ya wa : IsSqRoot Na ya wa =>
+  equiv [ZK(HP, V).main ~ Sim1'.simulate
+         : ={arg, glob V} /\ arg{1} = (Na, ya, wa)
+          ==> res{1} = res{2}.`2 ].
+move => isqr. proc.
+inline*. sp.
+call (_:true).
+wp. call (_:true).
+wp. swap {2} 2 -1.
+rnd. rnd {2}. skip. progress. 
+smt (d_prop2).
 qed.
 
 
-local lemma qkok Na ya P : IsQR Na ya =>
+
+local lemma exss Na ya wa : IsSqRoot Na ya wa => invertible Na ya =>
+ equiv[ Sim1.sinit ~ Sim1'.sinit
+   : ={arg} /\ arg{1} = (Na,ya) ==>
+       (res{1}.`1, res{1}.`2) = (res{2}.`1, res{2}.`2)
+        /\ (res{1}.`1 = true  => res{1}.`2 %% Na = res{1}.`3 * res{1}.`3 * (inv Na ya) %% Na
+                /\ res{1}.`3 * (inv Na wa) %% Na  = res{2}.`3 %% Na )
+        /\ (res{1}.`1 = false => res{1}.`2 %% Na = res{1}.`3 * res{1}.`3 %% Na
+                /\ res{1}.`2  = res{2}.`2 
+                /\ res{1}.`3  = res{2}.`3 ) ].
+move => isqr invrtbl. proc. swap 2 -1.
+seq 1 1 : (={N,y,bb} /\ (N{1},y{1}) = (Na,ya)). rnd. skip. auto.
+exists* bb{1}. elim*. progress.
+wp. case (bb_L = true).     
+rnd (fun (x : int * int) => (x.`1 * inv N{1} wa %% N{1}, x.`2 * (inv N{1} y{1}) %% N{1} ))
+      (fun (x : int * int) => (x.`1 * wa %% N{1}, x.`2 * y{1} %% N{1})). skip. progress.
+
+have ->: rrrR = (rrrR.`1 %% N{2}, rrrR.`2 %% N{2}). smt (d_prop2).
+simplify. split. 
+  have : invertible N{2} wa.  smt.
+move => iwa. 
+
+have ->:  rrrR.`1 %% N{2} * wa %% N{2} * inv N{2} wa %% N{2}
+ =  (rrrR.`1  * wa  * inv N{2} wa) %% N{2}.
+smt (modzMml modzMmr modzMm).
+have ->: rrrR.`1 * wa * inv N{2} wa = rrrR.`1 * (wa * inv N{2} wa).
+smt.
+smt (modzMml modzMmr modzMm qr_prop1).
+
+have ->:  rrrR.`2 %% N{2} * y{2} %% N{2} * inv N{2} y{2} %% N{2}
+ =  (rrrR.`2  * y{2}  * inv N{2} y{2}) %% N{2}.
+smt (modzMml modzMmr modzMm).
+have ->: rrrR.`2 * y{2} * inv N{2} y{2} = rrrR.`2 * (y{2} * inv N{2} y{2}).
+smt.
+smt (modzMml modzMmr modzMm qr_prop1).
+admit. 
+admit. 
+
+have ->: rrrL = (rrrL.`1 %% N{2}, rrrL.`2 %% N{2}). smt (d_prop2).
+simplify. split. 
+  have : invertible N{2} wa.  smt.
+move => iwa. 
+have ->:  rrrL.`1 %% N{2} *  inv N{2} wa %% N{2} * wa %% N{2}
+ =  (rrrL.`1  * inv N{2} wa * wa ) %% N{2}.
+smt (modzMml modzMmr modzMm).
+have ->: rrrL.`1 * inv N{2} wa * wa = rrrL.`1 * (wa * inv N{2} wa).
+smt.
+smt (modzMml modzMmr modzMm qr_prop1).
+have ->:  rrrL.`2 %% N{2} *  inv N{2} y{2} %% N{2} * y{2} %% N{2}
+ =  (rrrL.`2  * inv N{2} y{2} * y{2} ) %% N{2}.
+smt (modzMml modzMmr modzMm).
+have ->: rrrL.`2 * inv N{2} y{2} * y{2} = rrrL.`2 * (y{2} * inv N{2} y{2}).
+smt.
+smt (modzMml modzMmr modzMm qr_prop1).
+smt.
+have ->: rrrL.`2 * inv N{2} y{2} %% N{2} %% N{2} 
+  = rrrL.`2 * inv N{2} y{2} %% N{2} . smt.
+have ->:  rrrL.`2 * inv N{2} y{2} %% N{2}
+     = rrrL.`2 %%N{2} * inv N{2} y{2} %% N{2}. smt.  
+have <-: rrrL.`1 * rrrL.`1 %%N{2} = rrrL.`2 %%N{2} . smt.  
+smt (modzMml modzMmr modzMm d_prop1).
+smt. 
+rnd. skip. progress. smt. smt. smt.
+have ->: rrrL.`2  %% N{2} %% N{2} 
+  = rrrL.`2  %% N{2} . smt.
+smt (d_prop1).
+qed.
+
+
+local lemma qkok Na ya wa P : IsSqRoot Na ya wa => invertible Na ya =>
   equiv [ Sim1.simulate ~ Sim1'.simulate
-   : ={arg, glob V} /\ (Na,ya) = (N{1},y{1})
+   :   ={glob V} /\ (Na,ya) = (N{1},y{1}) /\ (Na,ya,wa) = (N{2},y{2},w{2})
        ==> (res{1}.`1 /\ P res{1}.`2) <=> (res{2}.`1 /\ P res{2}.`2) ].
-move => isqr. proc.
-seq 1 1 : (={N,y,glob V,b',z} /\ (b'{1} = true => z{1} = rr{1} * (inv Na ya)) /\ (b'{2} = false => z{1} = rr{1} /\ z{1} = z{2}) /\  (Na, ya) = (Na{2},y{2}) ).
-call (exss Na ya). skip. progress.
-seq 1 1 : (={b,N,y,glob V,b',z} /\ (b'{1} = true => z{1} = rr{1} * (inv Na ya)) /\ (b'{2} = false => z{1} = rr{1} /\ z{1} = z{2}) /\  (Na, ya) = (Na{2},y{2}) ).
+move => isqr invrtbl. proc.
+seq 1 1 : (={N,y,glob V,b',z} 
+         /\ (b'{1} = true => z{1} %% Na = r{1} * r{1} * (inv Na ya) %% Na
+                     /\ r{1} * (inv Na wa) %% Na = r{2} %% Na )
+         /\ (b'{2} = false => z{1} %% Na = r{1} * r{1} %% Na /\ r{1} = r{2})
+         /\ (Na, ya,wa) = (N{2},y{2},w{2}) ).
+
+call (exss Na ya wa). skip. progress. smt.  smt. 
+    
+seq 1 1 : (={b,N,y,glob V,b',z} 
+         /\ (b'{1} = true => z{1} %% Na = r{1} * r{1} * (inv Na ya) %% Na
+                     /\ r{1} * (inv Na wa) %% Na = r{2} %% Na )
+         /\ (b'{2} = false => z{1} %% Na = r{1} * r{1} %% Na /\ r{1} = r{2})
+         /\ (Na, ya,wa) = (N{2},y{2},w{2}) ).
+
+
 call (_:true). skip. progress.
 exists* b'{1}. elim*. progress.
 case (b'_L = true).
 exists* b{1}. elim*. progress.
 case (b_L = true).
-seq 1 1 : (={b,N,y,glob V,b',z,ryb}
-  /\ (b'{1} = true => z{1} = rr{1} * (inv Na ya))
-  /\ (b'{2} = false => z{1} = rr{1} /\ z{1} = z{2})
-  /\ (Na, ya) = (Na{2},y{2})).
-wp. skip. progress. rewrite H. auto. smt.
+    
+seq 1 1 : (={ryb,b,N,y,glob V,b',z} 
+         /\ (b'{1} = true => z{1} %% Na = r{1} * r{1} * (inv Na ya) %% Na
+                     /\ r{1} * (inv Na wa) %% Na = r{2} %% Na )
+         /\ (b'{2} = false => z{1} %% Na = r{1} * r{1} %% Na /\ r{1} = r{2})
+         /\ (Na, ya,wa) = (N{2},y{2},w{2}) ).
+
+
+wp. skip. progress.  
+  
+have : r{1} * inv N{2} w{2} %% N{2} = r{2} %% N{2}.  smt.
+move => qq. clear H H0. 
+
+have : r{1} * inv N{2} w{2} %% N{2} * w{2} = r{2} %% N{2} * w{2}.
+smt. clear qq. move => qq. 
+have : r{1} * inv N{2} w{2} %% N{2} * w{2} %% N{2} = r{2} %% N{2} * w{2} %% N{2}.
+smt. clear qq. move => qq.
+have : invertible N{2} w{2}. smt.
+move => iwa.
+
+have <-: r{1} * inv N{2} w{2} %% N{2} * w{2} %% N{2} = r{1} %% N{2}.
+  have ->: r{1} * inv N{2} w{2} %% N{2} * w{2} %% N{2}
+          = r{1} * inv N{2} w{2} * w{2} %% N{2}.
+smt (modzMml modzMmr modzMm qr_prop1).
+  have ->: r{1} * inv N{2} w{2} * w{2} = r{1} * (inv N{2} w{2} * w{2}).
+  smt .
+      smt (modzMml modzMmr modzMm qr_prop11).
+      smt (modzMml modzMmr modzMm ).
+
+         smt. smt.
 auto. call (_:true). skip. progress. sp.
 conseq (_: b{1} <> b'{1} ==> b{1} <> b'{1}). smt. smt.
 call {1}  (_: true ==> true). apply summitup_ll. 
@@ -248,38 +405,13 @@ wp. skip. auto.
 qed.
 
 
-module ZK(P : Prover, V : VerifierA) = {
-  proc main(N : int, y : int) = {
-    var c,b,r,result;
-    c <- P.commit(N, y);  
-    b <- V.challenge(N,y,c);
-    r <- P.response(b);
-    result <- V.summitup(c,b,r); 
-    return result;
-  }
-}.
 
-
-local lemma qrp_zk2_eq Na ya : IsQR Na ya =>
-  equiv [ZK(HP, V).main ~ Sim1'.simulate
-         : ={arg, glob V} /\ arg{1} = (Na, ya)
-          ==> res{1} = res{2}.`2 ].
-move => isqr. proc.
-inline*. sp.
-call (_:true).
-wp. call (_:true).
-wp. swap {2} 2 -1.
-rnd. rnd {2}. skip. progress.
-smt.
-qed.
-
-
-local lemma qrp_zk2_pr &m Na ya a : IsQR Na ya =>
-    Pr[ZK(HP, V).main(Na,ya) @ &m : res = a ] 
-     = Pr[ Sim1'.simulate(Na,ya) @ &m : res.`2 = a ].
+local lemma qrp_zk2_pr &m Na ya wa a : IsSqRoot Na ya wa =>
+    Pr[ZK(HP, V).main(Na,ya,wa) @ &m : res = a ] 
+     = Pr[ Sim1'.simulate(Na,ya,wa) @ &m : res.`2 = a ].
 proof. move => isqr. byequiv.
 conseq (_: _ ==> res{1} = res{2}.`2). progress.
-conseq (qrp_zk2_eq Na ya isqr). auto. auto. auto.
+conseq (qrp_zk2_eq Na ya wa isqr ). auto. auto. auto.
 qed.
 
 
